Convert ShowAST to DString.
- Add DList.v file for some difference list functions.
  + Trying to use as much tail recursion as possible
      in DLists to prevent stack performance problems.
- Add DString type (like string, but it uses difference lists)
- Convert show instances to use DString where possible.
  + Uses the new DShow typeclass and instances.

Additionally we added the QCShowTesting.v file

Compiling this file should cause a stack overflow with the old show
instances (that don't use diff lists for appends).

defSize can be changed to alter how large the programs we try to
generate are --- I am not sure if 50 is just too large or not. We may
have to compare the diff list version to the original version and see
what size tends to work for both of them. Ideally we should be able to
increase the size more with the diff list version :). Test cases are
randomly generated, so you may have to run the QuickChick command
multiple times to be sure (it may randomly decide to generate smaller programs).

src/coq/QC/GenAST.v
@@ -22,7 +22,7 @@ Require Import List.
 
 Import ListNotations.
 
-From Vellvm Require Import LLVMAst Utilities AstLib Syntax.CFG Syntax.TypeUtil Syntax.TypToDtyp DynamicTypes Semantics.TopLevel QC.Utils Handlers.Handlers.
+From Vellvm Require Import LLVMAst Utilities AstLib Syntax.CFG Syntax.TypeUtil Syntax.TypToDtyp DynamicTypes Semantics.TopLevel QC.Utils Handlers.Handlers DList.
 Require Import Integers.
 
 
@@ -43,45 +43,12 @@ From ExtLib.Structures Require Export
      Functor.
 Open Scope Z_scope.
 
-
 (* Disable guard checking. This file is only used for generating test
     cases. Some of our generation functions terminate in non-trivial
     ways, but since they're only used to generate test cases (and are
     not used in proofs) it's not terribly important to prove that they
     actually terminate.  *)
 Unset Guard Checking.
-(** Difference lists *)
-Section DList.
-  Definition DList (A : Type) := list A -> list A.
-
-  Definition DList_to_list {A} (dl : DList A) : list A
-    := dl [].
-
-  Definition DList_append {A} (dl1 dl2 : DList A) : DList A
-    := fun xs => dl1 (dl2 xs).
-
-  Definition DList_singleton {A} (a : A) : DList A
-    := cons a.
-
-  Definition DList_cons {A} (a : A) (dl : DList A) : DList A
-    := DList_append (DList_singleton a) dl.
-
-  Definition DList_empty {A} : DList A
-    := fun xs => xs.
-
-  Definition DList_from_list {A} (l : list A) : DList A
-    := fold_right DList_cons DList_empty l.
-
-  Definition DList_map {A B} (f : A -> B) (dl : DList A) : DList B
-    := fold_right (fun a => DList_cons (f a)) (@DList_empty B) (DList_to_list dl).
-
-  #[global] Instance DList_Functor : Functor DList.
-  Proof.
-    split.
-    intros A B X X0.
-    eapply DList_map; eauto.
-  Defined.
-End DList.
 
 Section Helpers.
   Fixpoint is_sized_type_h (t : typ) : bool
