src/coq/QC/ShowAST.v
@@ -4,8 +4,7 @@
     program should give you a string that can be read by clang.
  *)
 
-
-From Vellvm Require Import LLVMAst Utilities AstLib Syntax.CFG DynamicTypes.
+From Vellvm Require Import LLVMAst Utilities AstLib Syntax.CFG DynamicTypes DList.
 
 Require Import Integers Floats.
 
@@ -32,67 +31,92 @@ Fixpoint concatStr (l : list string) : string :=
 (*  ------------------------------------------------------------------------- *)
 
 
+Class DShow (A : Type) := { dshow : A -> DString }.
+
+#[global] Infix "@@" := (DList_append) (right associativity, at level 60).
+
+#[global] Instance DShowList {A} `{DShow A} : DShow (list A) :=
+  { dshow := fun x => DList_join (map dshow x) }.
+
+#[global] Instance DShowPair {A B : Type} `{_ : DShow A} `{_ : DShow B} : DShow (A * B) :=
+{|
+  dshow p := match p with (a,b) => string_to_DString "(" @@ dshow a @@ string_to_DString "," @@ dshow b @@ string_to_DString ")" end
+|}.
+
+#[global] Instance DShowShow {A} `{DShow A} : Show A :=
+{|
+  show a := DString_to_string (dshow a);
+|}.
+
 Section ShowInstances.
   Local Open Scope string.
 
-  Context {T:Set}.
-  Context `{Show T}.
+  Context {T : Set}.
+  Context `{DShow T}.
 
-
-  Definition show_raw_id (rid : raw_id) : string
+  Definition dshow_raw_id (rid : raw_id) : DString
     := match rid with
-       | Name s => s
-       | Anon i => show i
-       | Raw i  => show i
+       | Name s => string_to_DString s
+       | Anon i => string_to_DString (show i)
+       | Raw i  => string_to_DString (show i)
        end.
 
-  #[global] Instance showRawId : Show raw_id
-    := {| show := show_raw_id |}.
+  #[global] Instance dshowRawId : DShow raw_id
+    := {| dshow := dshow_raw_id |}.
 
-  Definition show_ident (i : ident) : string
+  Definition dshow_ident (i : ident) : DString
     := match i with
-       | ID_Global r => "@" ++ show_raw_id r
-       | ID_Local r  => "%" ++ show_raw_id r
+      | ID_Global r => string_to_DString "@" @@ dshow_raw_id r
+      | ID_Local r  => string_to_DString "%" @@ dshow_raw_id r
        end.
 
-  #[global] Instance showIdent : Show ident
-    := {| show := show_ident |}.
+  #[global] Instance dshowIdent : DShow ident
+    := {| dshow := dshow_ident |}.
 
-
-  Fixpoint show_typ (t : typ) : string :=
+  Fixpoint dshow_typ (t : typ) : DString  :=
     match t with
-    | TYPE_I sz                 => "i" ++ show sz
-    | TYPE_IPTR                 => "iptr"
-    | TYPE_Pointer t            => show_typ t ++ "*"
-    | TYPE_Void                 => "void"
-    | TYPE_Half                 => "half"
-    | TYPE_Float                => "float"
-    | TYPE_Double               => "double"
-    | TYPE_X86_fp80             => "x86_fp80"
-    | TYPE_Fp128                => "fp128"
-    | TYPE_Ppc_fp128            => "ppc_fp128"
-    | TYPE_Metadata             => "metadata"
-    | TYPE_X86_mmx              => "x86_mmx"
-    | TYPE_Array sz t           => "[" ++ show sz ++ " x " ++ show_typ t ++ "]"
+    | TYPE_I sz                 => string_to_DString "i" @@
+                                    string_to_DString (show sz)
+    | TYPE_IPTR                 => string_to_DString "iptr"
+    | TYPE_Pointer t            => dshow_typ t @@ string_to_DString "*"
+    | TYPE_Void                 => string_to_DString "void"
+    | TYPE_Half                 => string_to_DString "half"
+    | TYPE_Float                => string_to_DString "float"
+    | TYPE_Double               => string_to_DString "double"
+    | TYPE_X86_fp80             => string_to_DString "x86_fp80"
+    | TYPE_Fp128                => string_to_DString "fp128"
+    | TYPE_Ppc_fp128            => string_to_DString "ppc_fp128"
+    | TYPE_Metadata             => string_to_DString "metadata"
+    | TYPE_X86_mmx              => string_to_DString "x86_mmx"
+    | TYPE_Array sz t           =>
+        list_to_DString ["["; show sz; " x "] @@ dshow_typ t @@
+        string_to_DString "]"
     | TYPE_Function ret args varargs =>
         let varargs_str :=
           if Nat.eqb (List.length args) 0 then
-            (if varargs then "..." else "")
+            (if varargs then string_to_DString "..." else string_to_DString  "")
           else
-            (if varargs then ", ..." else "")
-        in
-        show_typ ret ++ " (" ++ concat ", " (map show_typ args) ++ varargs_str ++ ")"
-    | TYPE_Struct fields        => "{" ++ concat ", " (map show_typ fields) ++ "}"
-    | TYPE_Packed_struct fields => "<{" ++ concat ", " (map show_typ fields) ++ "}>"
-    | TYPE_Opaque               => "opaque"
-    | TYPE_Vector sz t          => "<" ++ show sz ++ " x " ++ show_typ t ++ ">"
-    | TYPE_Identified id        => show id
+            (if varargs then string_to_DString ", ..." else string_to_DString "")
+        in dshow_typ ret @@ string_to_DString  " (" @@
+           concat_DString (string_to_DString ", ") (map dshow_typ args) @@ varargs_str @@ string_to_DString ")"
+
+    | TYPE_Struct fields        => string_to_DString "{" @@
+                                   concat_DString (string_to_DString ", ") (map dshow_typ fields) @@
+                                   string_to_DString "}"
+    | TYPE_Packed_struct fields =>
+        string_to_DString "<{" @@ concat_DString (string_to_DString ", ") (map dshow_typ fields) @@
+        string_to_DString "}>"
+
+    | TYPE_Opaque               => string_to_DString "opaque"
+    | TYPE_Vector sz t          => string_to_DString "<" @@
+                                   string_to_DString (show sz) @@
+                                   string_to_DString " x " @@ dshow_typ t @@
+                                   string_to_DString ">"
+    | TYPE_Identified id        => dshow id
     end.
 
-  #[global] Instance showTyp:  Show typ :=
-    {|
-      show := show_typ
-    |}.
+  #[global] Instance dshowTyp : DShow typ :=
+    {| dshow := dshow_typ |}.
 
   Definition show_dtyp (t : dtyp) : string
     := match t with
@@ -133,7 +157,6 @@ Section ShowInstances.
   #[global] Instance showLinkage : Show linkage
     := {| show := show_linkage |}.
 
-
   Definition show_dll_storage (d : dll_storage) : string :=
     match d with
     | DLLSTORAGE_Dllimport => "dllimport"
@@ -173,39 +196,41 @@ Section ShowInstances.
   #[global] Instance showCConv : Show cconv
     := {| show := show_cconv |}.
 
-  Definition show_param_attr (p : param_attr) : string :=
+  Definition show_param_attr (p : param_attr) : DString :=
     match p with
-    | PARAMATTR_Zeroext => "zeroext"
-    | PARAMATTR_Signext => "signext"
-    | PARAMATTR_Inreg => "inreg"
-    | PARAMATTR_Byval t => "byval(" ++ show t ++ ")"
-    | PARAMATTR_Byref t => "byref(" ++ show t ++ ")"
-    | PARAMATTR_Preallocated t => "preallocated(" ++ show t ++ ")"
-    | PARAMATTR_Inalloca t => "inalloca(" ++ show t ++ ")"
-    | PARAMATTR_Sret t => "sret(" ++ show t ++ ")"
-    | PARAMATTR_Elementtype t => "elementtype(" ++ show t ++ ")"
-    | PARAMATTR_Align a => "align " ++ show a
-    | PARAMATTR_Noalias => "noalias"
-    | PARAMATTR_Nocapture => "nocapture"
-    | PARAMATTR_Readonly => "readonly"
-    | PARAMATTR_Nofree => "nofree"
-    | PARAMATTR_Nest => "nest"
-    | PARAMATTR_Returned => "returned"
-    | PARAMATTR_Nonnull => "nonnull"
-    | PARAMATTR_Dereferenceable a => "dereferenceable(" ++ show a ++ ")"
-    | PARAMATTR_Dereferenceable_or_null a => "dereferenceable_or_null(" ++ show a ++ ")"
-    | PARAMATTR_Swiftself => "swiftself"
-    | PARAMATTR_Swiftasync => "swiftasync"
-    | PARAMATTR_Swifterror => "swifterror"
-    | PARAMATTR_Immarg => "immarg"
-    | PARAMATTR_Noundef => "noundef"
-    | PARAMATTR_Alignstack a => "alignstack(" ++ show a ++ ")"
-    | PARAMATTR_Allocalign => "allocalign"
-    | PARAMATTR_Allocptr => "allocptr"
+    | PARAMATTR_Zeroext => string_to_DString "zeroext"
+    | PARAMATTR_Signext => string_to_DString "signext"
+    | PARAMATTR_Inreg => string_to_DString "inreg"
+    | PARAMATTR_Byval t => string_to_DString "byval(" @@ dshow t @@ string_to_DString ")"
+    | PARAMATTR_Byref t => string_to_DString "byref(" @@ dshow t @@ string_to_DString ")"
+    | PARAMATTR_Preallocated t => string_to_DString "preallocated(" @@ dshow t @@ string_to_DString ")"
+    | PARAMATTR_Inalloca t => string_to_DString "inalloca(" @@ dshow t @@ string_to_DString ")"
+    | PARAMATTR_Sret t => string_to_DString "sret(" @@ dshow t @@ string_to_DString ")"
+    | PARAMATTR_Elementtype t => string_to_DString "elementtype(" @@ dshow t @@ string_to_DString ")"
+    | PARAMATTR_Align a => string_to_DString "align " @@ string_to_DString (show a)
+    | PARAMATTR_Noalias => string_to_DString "noalias"
+    | PARAMATTR_Nocapture => string_to_DString "nocapture"
+    | PARAMATTR_Readonly => string_to_DString "readonly"
+    | PARAMATTR_Nofree => string_to_DString "nofree"
+    | PARAMATTR_Nest => string_to_DString "nest"
+    | PARAMATTR_Returned => string_to_DString "returned"
+    | PARAMATTR_Nonnull => string_to_DString "nonnull"
+    | PARAMATTR_Dereferenceable a => string_to_DString "dereferenceable(" @@ string_to_DString (show a) @@
+                                    string_to_DString ")"
+    | PARAMATTR_Dereferenceable_or_null a => string_to_DString "dereferenceable_or_null(" @@
+                                            string_to_DString (show a) @@ string_to_DString ")"
+    | PARAMATTR_Swiftself => string_to_DString "swiftself"
+    | PARAMATTR_Swiftasync => string_to_DString "swiftasync"
+    | PARAMATTR_Swifterror => string_to_DString "swifterror"
+    | PARAMATTR_Immarg => string_to_DString "immarg"
+    | PARAMATTR_Noundef => string_to_DString "noundef"
+    | PARAMATTR_Alignstack a => string_to_DString "alignstack(" @@ string_to_DString (show a)  @@ string_to_DString ")"
+    | PARAMATTR_Allocalign => string_to_DString "allocalign"
+    | PARAMATTR_Allocptr => string_to_DString "allocptr"
     end.
 
-  #[global] Instance showParamAttr : Show param_attr
-    := { show := show_param_attr }.
+  #[global] Instance dshowParamAttr : DShow param_attr
+    := { dshow := show_param_attr }.
 
   Definition show_fn_attr (f : fn_attr) : string :=
     match f with
@@ -440,7 +465,7 @@ Section ShowInstances.
        | Fast => "fast"
        end.
 
-  #[global] Instance showFastMatch : Show fast_math
+  #[global] Instance showFastMath : Show fast_math
     := {| show := show_fast_math |}.
 
   (*These are Constant Expressions*)
@@ -490,8 +515,22 @@ Section ShowInstances.
     else if (n =? 34)%nat then "\22"
     (*Special case for decimal 92/hex 5C*)
     else if (n =? 92)%nat then "\\"
-    else (string_of_list_ascii ((ascii_of_nat n) :: [])).
+         else (string_of_list_ascii ((ascii_of_nat n) :: [])).
 
+  Definition dshow_c_string (ex : exp T) : DString :=
+    let n : nat := ex_to_nat ex in
+    let x : Z := ex_to_int ex in
+    if ((n <? 32) || (126 <? n))%nat then (
+        let conversion_str := NilEmpty.string_of_uint (N.to_hex_uint (Z.to_N x)) in
+        let conversion := NilEmpty.string_of_uint (N.to_hex_uint (Z.to_N x)) in
+        if ((length conversion_str) =? (Z.to_nat 1))%nat then string_to_DString "\0" @@ string_to_DString conversion
+        else string_to_DString "\" @@ string_to_DString conversion
+      )
+    (*Special case for decimal 34/hex 22*)
+    else if (n =? 34)%nat then string_to_DString "\22"
+    (*Special case for decimal 92/hex 5C*)
+    else if (n =? 92)%nat then string_to_DString "\\"
+         else DList_cons (ascii_of_nat n) DList_empty.
 
   Definition is_op (e : exp T) : bool :=
     match e with
@@ -514,106 +553,163 @@ tes on cstring on LLVMAst.v *)
     | _ => true
     end.
 
-  Definition add_parens (b : bool) (s : string) : string :=
-    if b then "(" ++ s ++ ")" else s.
+  Definition add_parens (b : bool) (ds : DString) : DString :=
+    if b then string_to_DString "(" @@ ds @@ string_to_DString ")" else ds.
 
-  Fixpoint show_exp (b: bool) (v : exp T) :=
-
+  Fixpoint dshow_exp (b: bool) (v : exp T) : DString :=
     match v with
-    | EXP_Ident id => show id
-    | EXP_Integer x => show x
-    | EXP_Float f => show f
-    | EXP_Double f => show f
-    | EXP_Hex f => double_to_hex_string f
-    | EXP_Bool b => show b
-    | EXP_Null => "null"
-    | EXP_Zero_initializer => "zeroinitializer"
+    | EXP_Ident id => dshow id
+    | EXP_Integer x => string_to_DString (show x)
+    | EXP_Float f => string_to_DString (show f)
+    | EXP_Double f => string_to_DString (show f)
+    | EXP_Hex f => string_to_DString (double_to_hex_string f)
+    | EXP_Bool b => string_to_DString (show b)
+    | EXP_Null => string_to_DString "null"
+    | EXP_Zero_initializer => string_to_DString "zeroinitializer"
     (* see notes on cstring on LLVMAst.v *)
     (* I'm using string_of_list_ascii bc I couldn't find any other function that converted asciis to strings  *)
-    | EXP_Cstring elts => "c" ++ """" ++
-                             concat "" (map (fun '(ty,ex) => show_c_string ex) elts)  ++ """"
-    | EXP_Undef => "undef"
-    | EXP_Struct fields => "{"  ++ concat ", " (map (fun '(ty,ex) => show ty ++ " " ++  show_exp false ex) fields) ++ "}"
-    | EXP_Packed_struct fields => "<{"  ++ concat ", " (map (fun '(ty,ex) => show ty ++ " " ++  show_exp false ex) fields) ++ "}>"
-    | EXP_Array elts => "["  ++ concat ", " (map (fun '(ty,ex) => show ty ++ " " ++  show_exp false ex) elts) ++ "]"
-    | EXP_Vector elts => "<"  ++ concat ", " (map (fun '(ty,ex) => show ty ++ " " ++  show_exp false ex) elts) ++ ">"
+    | EXP_Cstring elts => string_to_DString "c" @@ string_to_DString """" @@
+                           DList_join (map (fun '(ty, ex) => (dshow_c_string ex)) elts) @@ string_to_DString  """"
+
+    | EXP_Undef => string_to_DString "undef"
+
+    | EXP_Struct fields =>
+        string_to_DString "{" @@
+          concat_DString (string_to_DString ", ")
+          (map (fun '(ty, ex) =>
+                  DList_join [dshow ty ; string_to_DString " "] @@
+                    dshow_exp false ex) fields) @@ string_to_DString "}"
+
+    | EXP_Packed_struct fields =>
+        string_to_DString "<{" @@
+          concat_DString (string_to_DString ", ")
+          (map (fun '(ty, ex) =>
+                  DList_join [dshow ty ; string_to_DString " "] @@
+                    dshow_exp false ex) fields) @@ string_to_DString "}>"
+
+    | EXP_Array elts =>
+        string_to_DString "[" @@
+          concat_DString (string_to_DString ", ")
+          (map (fun '(ty, ex) => DList_join [dshow ty ; string_to_DString " "] @@ dshow_exp false ex) elts) @@ string_to_DString "]"
+    | EXP_Vector elts => string_to_DString "<" @@ concat_DString (string_to_DString ", ") (map (fun '(ty, ex) => DList_join [dshow ty ; string_to_DString " "] @@ dshow_exp false ex) elts) @@ string_to_DString ">"
+
     | OP_IBinop iop t v1 v2 =>
-       let second_expression :=  if b then  show t ++ " " ++ show_exp true v2 else show_exp true v2 in
-       show iop ++ " " ++ add_parens b (show t ++ " " ++  show_exp true v1 ++ ", " ++ second_expression)
+        let second_expression :=
+          if b
+          then dshow t @@ string_to_DString " " @@ dshow_exp true v2
+          else dshow_exp true v2
+       in string_to_DString (show iop) @@ string_to_DString " " @@ add_parens b (dshow t @@ string_to_DString " " @@ dshow_exp true v1 @@ string_to_DString ", " @@ second_expression)
+
     | OP_ICmp cmp t v1 v2 =>
-        let second_expression :=  if b then  show t ++ " " ++ show_exp true v2 else show_exp true v2 in
-        "icmp " ++  show cmp ++ " " ++  add_parens b (show t ++ " " ++  show_exp true v1 ++ ", " ++ second_expression)
+        let second_expression :=
+          if b
+          then dshow t @@ string_to_DString " " @@ dshow_exp true v2
+          else dshow_exp true v2
+        in list_to_DString ["icmp " ; show cmp ; " "] @@ add_parens b (dshow t @@ string_to_DString " " @@ dshow_exp true v1 @@ string_to_DString ", " @@ second_expression)
+
     | OP_FBinop fop fmath t v1 v2 =>
         let fmath_string :=
-          match fmath with
-          | nil => " "
-          | _ =>  " " ++ concat " " (map (fun x => show x) fmath) ++  " "
-          end in
-        show fop ++ " " ++ add_parens b (fmath_string ++ show t ++ " " ++  show_exp true v1 ++ ", " ++  show_exp true v2)
-    | OP_FCmp cmp t v1 v2 =>
-        "fcmp " ++  add_parens b (show cmp ++ " " ++ show t ++ " " ++  show_exp true v1 ++ ", " ++  show_exp true v2)
-    | OP_Conversion conv t_from v t_to => show conv ++ " " ++ add_parens b (show t_from ++ " " ++  show_exp true v ++ " to " ++ show t_to)
-   | OP_GetElementPtr t ptrval idxs =>
-        let (tptr, exp) := ptrval in
+          string_to_DString
+            match fmath with
+            | nil => " "
+            | _ =>  " " ++ concat " " (map (fun x => show x) fmath) ++  " "
+            end
+        in list_to_DString [show fop ; " "] @@ add_parens b (fmath_string @@ dshow t @@ string_to_DString " " @@  dshow_exp true v1 @@ string_to_DString ", " @@ dshow_exp true v2)
 
-       "getelementptr " ++  add_parens b (show t ++ ", " ++ show tptr ++ " " ++ show_exp true exp ++  fold_left (fun str '(ty, ex) => str ++ ", " ++ show ty ++ " " ++ show_exp true ex) idxs "")
+    | OP_FCmp cmp t v1 v2 =>
+        string_to_DString "fcmp " @@ add_parens b (list_to_DString [show cmp ; " "] @@ dshow t @@ string_to_DString " " @@ dshow_exp true v1 @@
+                                                 string_to_DString ", " @@ dshow_exp true v2)
+
+    | OP_Conversion conv t_from v t_to => list_to_DString [show conv ; " "] @@ add_parens b (dshow t_from @@ string_to_DString " " @@ dshow_exp true v @@
+                                                                                             string_to_DString " to " @@ dshow t_to)
+
+    | OP_GetElementPtr t ptrval idxs =>
+        let (tptr, exp) := ptrval in
+        string_to_DString "getelementptr " @@ add_parens b (dshow t @@ string_to_DString ", " @@ dshow tptr @@ string_to_DString " " @@ dshow_exp true exp @@
+                                                              fold_left (fun str '(ty, ex) => str @@ string_to_DString ", " @@ dshow ty @@ string_to_DString " " @@ dshow_exp true ex) idxs DList_empty)
 
     | OP_ExtractElement vec idx =>
         let (tptr, exp) := vec in
         let (tidx, iexp) := idx in
-        "extractelement " ++  add_parens b ( show tptr ++ " " ++  show_exp true exp ++ ", " ++ show tidx ++ " " ++  show_exp true iexp)
+        string_to_DString "extractelement " @@ add_parens b (dshow tptr @@ string_to_DString " " @@ dshow_exp true exp @@ string_to_DString ", " @@ dshow tidx @@ string_to_DString " " @@  dshow_exp true iexp)
+
     | OP_InsertElement vec elt idx =>
         let (tptr, exp) := vec in
         let (telt, eexp) := elt in
         let (tidx, iexp) := idx in
-         "insertelement " ++ add_parens b (show tptr ++ " " ++  show_exp true exp ++ ", " ++ show telt ++ " " ++  show_exp true eexp ++ ", " ++ show tidx ++ " " ++ show_exp true iexp)
+        string_to_DString "insertelement " @@ add_parens b (dshow tptr @@ string_to_DString " " @@ dshow_exp true exp @@ string_to_DString ", " @@ dshow telt @@ string_to_DString " " @@
+                                                          dshow_exp true eexp @@ string_to_DString ", " @@ dshow tidx @@ string_to_DString " " @@ dshow_exp true iexp)
+
     | OP_ShuffleVector vec1 vec2 idxmask =>
         let (type1, expression1) := vec1 in
         let (type2, expression2) := vec2 in
         let (type3, expression3) := idxmask in
-        "shufflevector " ++  add_parens b (show type1 ++  show_exp true expression1  ++ ", " ++ show type2 ++  show_exp true expression2 ++ ", " ++ show type3 ++  show_exp true expression3)
+        string_to_DString "shufflevector " @@ add_parens b (dshow type1 @@ dshow_exp true expression1 @@ string_to_DString ", " @@ dshow type2 @@ dshow_exp true expression2 @@
+                                                              string_to_DString ", " @@ dshow type3 @@ dshow_exp true expression3)
     (* This one, extractValue *)
     | OP_ExtractValue vec idxs =>
         let (tptr, exp) := vec in
-       "extractvalue " ++  add_parens b ( show tptr ++ " " ++  show_exp true exp ++ ", " ++ concat ", " (map (fun x => show x) idxs))
+        string_to_DString "extractvalue " @@ add_parens b (dshow tptr @@ string_to_DString " " @@ dshow_exp true exp @@ string_to_DString ", " @@
+                                                         concat_DString (string_to_DString ", ") (map (fun x => string_to_DString (show x)) idxs))
+
+
     | OP_InsertValue vec elt idxs =>
         let (tptr, exp) := vec in
         let (telt, eexp) := elt in
-        "insertvalue " ++  add_parens b (show tptr ++ " " ++  show_exp false exp ++ ", " ++ show telt ++ " " ++  show_exp false eexp ++ ", " ++ concat ", " (map (fun x => show x) idxs))
+        string_to_DString "insertvalue " @@ add_parens b (dshow tptr @@ string_to_DString " " @@ dshow_exp false exp @@ string_to_DString ", " @@ dshow telt @@ string_to_DString " " @@
+                                                            dshow_exp false eexp @@ string_to_DString ", " @@ concat_DString (string_to_DString ", ") (map (fun x => string_to_DString (show x)) idxs))
+
     | OP_Select (tc, cnd) (t1, v1) (t2, v2) =>
-        "select "  ++  add_parens b (show tc ++ " " ++  show_exp true cnd ++ ", " ++ show t1 ++ " " ++  show_exp true v1  ++ ", " ++ show t2 ++ " " ++  show_exp true v2)
-    | OP_Freeze (ty, ex) => "freeze " ++ add_parens b (show ty ++ " " ++ show_exp true ex)
+        string_to_DString "select "  @@ add_parens b (dshow tc @@ string_to_DString " " @@ dshow_exp true cnd @@ string_to_DString ", " @@ dshow t1 @@ string_to_DString " " @@
+                                                    dshow_exp true v1  @@ string_to_DString ", " @@ dshow t2 @@ string_to_DString " " @@  dshow_exp true v2)
+
+    | OP_Freeze (ty, ex) => string_to_DString "freeze " @@ add_parens b (dshow ty @@ string_to_DString " " @@ dshow_exp true ex)
     end.
 
+  #[global] Instance dshowExp : DShow (exp T) :=
+    {| dshow := dshow_exp false |}.
 
-  #[global] Instance showExp : Show (exp T)
-    := {| show := show_exp false |}.
+  #[global] Instance dshowTEXP : DShow (texp T) :=
+    {| dshow te := let '(t, e) := te in dshow t @@ string_to_DString " "
+                              @@ dshow e |}.
 
-  #[global] Instance showTExp : Show (texp T)
-    := {| show te :=
-         match te with
-         | (t, e) => show t ++ " " ++ show e
-         end
-       |}.
+  #[global] Instance dshowTExp : DShow (texp T)
+    := {| dshow te := let '(t, e) := te in dshow t @@ string_to_DString " " @@ dshow e |}.
 
-  Definition show_phi_block (p : block_id * exp T) : string :=
+  Definition show_phi_block (p : block_id * exp T) : DString :=
     let '(bid, e) := p in
-    "[ " ++ show_exp true e ++ ", " ++ "%" ++ show bid ++ " ]".
+    string_to_DString "[ " @@ dshow_exp true e @@ list_to_DString [", "; "%"] @@ dshow bid @@ string_to_DString " ]".
 
   Definition intersperse (sep : string) (l : list string) : string
     := fold_left (fun acc s => if StringOrdFacts.eqb "" acc then s else acc ++ sep ++ s) l "".
 
-  #[global] Instance showPhi : Show (phi T)
-    := {| show p :=
-         let '(Phi t phis) := p in
-         "phi " ++ show t ++ " " ++ intersperse ", " (map show_phi_block phis)
-       |}.
+  Definition dintersperse (sep : DString) (l : list DString) : DString
+    := fold_left (fun acc s => if StringOrdFacts.eqb "" (DString_to_string acc) then s else acc @@ sep @@ s) l (string_to_DString "").
 
+  Fixpoint dconcat (sep : DString) (ls : list DString) :=
+    match ls with
+    | nil => string_to_DString EmptyString
+    | cons x nil => x
+    | cons x xs => x @@ sep @@ dconcat sep xs
+    end.
+
+  #[global] Instance dshowPhi : DShow (phi T)
+    := {| dshow p :=
+         let '(Phi t phis) := p in
+         DList_join [string_to_DString "phi " ; dshow t ; string_to_DString " "] @@
+           concat_DString (string_to_DString ", ") (map show_phi_block phis)
+       |}.
 
   Definition show_opt_prefix {A} `{Show A} (prefix : string) (ma : option A) : string
     := match ma with
        | None   => ""
        | Some a => prefix ++ show a
+       end.
+
+  Definition dshow_opt_prefix {A} `{DShow A} (prefix : DString) (ma : option A) : DString
+    := match ma with
+       | None   => string_to_DString ""
+       | Some a => prefix @@ dshow a
        end.
 
   Definition show_opt_list {A} `{Show A} (ma : option A) : list string
@@ -622,42 +718,73 @@ tes on cstring on LLVMAst.v *)
        | Some a => [show a]
        end.
 
+  Definition dshow_opt_list {A} `{DShow A} (ma : option A) : list DString
+    := match ma with
+       | None   => []
+       | Some a => [dshow a]
+       end.
 
-  Definition show_ordering (o : ordering) : string :=
-    match o with
-    |Unordered => "unordered"
-    |Monotonic => "monotonic"
-    |Acquire => "acquire"
-    |Release => "release"
-    |Acq_rel => "acq_rel"
-    |Seq_cst => "seq_cst"
-    end.
+  Definition show_ordering (o : ordering) : DString :=
+    string_to_DString
+      match o with
+      |Unordered => "unordered"
+      |Monotonic => "monotonic"
+      |Acquire => "acquire"
+      |Release => "release"
+      |Acq_rel => "acq_rel"
+      |Seq_cst => "seq_cst"
+      end.
 
-  #[global] Instance showOrdering : Show (ordering)
-    := {| show := show_ordering |}.
+  #[global] Instance dshowOrdering : DShow (ordering)
+    := {| dshow := show_ordering |}.
 
-  Definition show_cmpxchg (c : cmpxchg T) : string :=
-    let p_weak := match c.(c_weak) with
-                  |None => ""
-                  |Some x => show x
-                  end in
-    let p_volatile := match c.(c_volatile) with
-                      |None => ""
-                      |Some x => show x
-                      end in
-    let p_syncscope := match c.(c_syncscope) with
-                       |None => ""
-                       |Some x => "[syncscope(""" ++ show x ++ """)]"
-                       end in
-    let p_align := match c.(c_align) with
-                   |None => ""
-                   |Some x => ", align " ++ show x
-                   end in
+  Definition show_cmpxchg (c : cmpxchg T) : DString :=
+    let p_weak :=
+      string_to_DString
+        match c.(c_weak) with
+        |None => ""
+        |Some x => show x
+        end in
+    let p_volatile :=
+      string_to_DString
+        match c.(c_volatile) with
+        |None => ""
+        |Some x => show x
+        end in
+    let p_syncscope :=
+      string_to_DString
+        match c.(c_syncscope) with
+        |None => ""
+        |Some x => "[syncscope(""" ++ show x ++ """)]"
+        end in
+    let p_align :=
+      string_to_DString
+        match c.(c_align) with
+        |None => ""
+        |Some x => ", align " ++ show x
+        end in
 
-    concatStr ["cmpxchg "; p_weak; p_volatile; show c.(c_ptr); ", ";  show c.(c_cmp_type); show c.(c_cmp); ", " ; show c.(c_new) ; p_syncscope ; show c.(c_success_ordering); show c.(c_failure_ordering) ; p_align ;  "yields  { "; show c.(c_cmp_type) ; ", i1 } "].
+    DList_join
+      [string_to_DString "cmpxchg ";
+       p_weak;
+       p_volatile;
+       dshow c.(c_ptr);
+       string_to_DString ", ";
+       dshow c.(c_cmp_type);
+       string_to_DString (show c.(c_cmp));
+       string_to_DString ", " ;
+       dshow c.(c_new);
+       p_syncscope;
+       dshow c.(c_success_ordering);
+       dshow c.(c_failure_ordering);
+       p_align;
+       string_to_DString "yields  { ";
+       dshow c.(c_cmp_type);
+       string_to_DString ", i1 } "
+      ].
 
-  #[global] Instance showCmpxchg : Show (cmpxchg T)
-    := {| show := show_cmpxchg |}.
+  #[global] Instance dshowCmpxchg : DShow (cmpxchg T)
+    := {| dshow := show_cmpxchg |}.
 
   Definition show_a_rmw_operation (a :  atomic_rmw_operation) : string :=
     match a with
@@ -679,7 +806,7 @@ tes on cstring on LLVMAst.v *)
   #[global] Instance showARmwOperation : Show (atomic_rmw_operation)
     := {| show := show_a_rmw_operation |}.
 
-  Definition show_atomic_rmw (a : atomicrmw T) : string :=
+  Definition show_atomic_rmw (a : atomicrmw T) : DString :=
     let p_volatile := match a.(a_volatile) with
                       |None => ""
                       |Some x => show x
@@ -694,34 +821,47 @@ tes on cstring on LLVMAst.v *)
                    |Some x => ", align " ++ show x
                    end in
 
-    concatStr ["atomicrmw" ;  p_volatile ; show a.(a_operation) ; show a.(a_ptr) ; ", " ;
-               show a.(a_val) ; p_syncscope ; show a.(a_ordering) ; p_align ; "yields " ;
-               show a.(a_type)].
+    DList_join
+      [string_to_DString "atomicrmw";
+       string_to_DString p_volatile;
+       string_to_DString (show a.(a_operation));
+       dshow a.(a_ptr);
+       string_to_DString ", ";
+       dshow a.(a_val);
+       string_to_DString p_syncscope;
+       dshow a.(a_ordering);
+       string_to_DString p_align;
+       string_to_DString "yields ";
+       dshow a.(a_type)].
 
-  #[global] Instance showAtomicrmw : Show (atomicrmw T)
-    := {| show := show_atomic_rmw |}.
+  #[global] Instance showAtomicrmw : DShow (atomicrmw T)
+    := {| dshow := show_atomic_rmw |}.
 
-
-  Fixpoint show_metadata (md : metadata T)  : string :=
+  Fixpoint dshow_metadata (md : metadata T)  : DString :=
     match md with
-    | METADATA_Const tv => show tv
-    | METADATA_Null => "null"
-    | METADATA_Nontemporal => "!nontemporal"
-    | METADATA_Invariant_load => "!invariant.load"
-    | METADATA_Invariant_group => "!invariant.group"
-    | METADATA_Nonnull => "!nonnull"
-    | METADATA_Dereferenceable => "!dereferenceable"
-    | METADATA_Dereferenceable_or_null => "!dereferenceable_or_null"
-    | METADATA_Align => "!align"
-    | METADATA_Noundef => "!noundef"
-    | METADATA_Id i => "!" ++ show i
-    | METADATA_String s => "!" ++ show s
-    | METADATA_Named strs => "!{" ++ intersperse " , " (List.map (fun x => "!" ++ x) strs) ++ "}"
-    | METADATA_Node mds => "!{" ++ intersperse " , " (List.map show_metadata mds) ++ "}"
+    | METADATA_Const tv => dshow tv
+    | METADATA_Null => string_to_DString "null"
+    | METADATA_Nontemporal => string_to_DString "!nontemporal"
+    | METADATA_Invariant_load => string_to_DString "!invariant.load"
+    | METADATA_Invariant_group => string_to_DString "!invariant.group"
+    | METADATA_Nonnull => string_to_DString "!nonnull"
+    | METADATA_Dereferenceable => string_to_DString "!dereferenceable"
+    | METADATA_Dereferenceable_or_null => string_to_DString "!dereferenceable_or_null"
+    | METADATA_Align => string_to_DString "!align"
+    | METADATA_Noundef => string_to_DString "!noundef"
+    | METADATA_Id i => string_to_DString "!" @@ dshow i
+    | METADATA_String s => string_to_DString "!" @@ string_to_DString (show s)
+    | METADATA_Named strs => string_to_DString "!{" @@
+                              concat_DString (string_to_DString " , ") (map (fun x => string_to_DString "!" @@
+                                                                                     string_to_DString x) strs)
+                              @@ string_to_DString "}"
+    | METADATA_Node mds => string_to_DString "!{"
+                            @@ concat_DString (string_to_DString " , ") (map dshow_metadata mds)
+                            @@ string_to_DString "}"
     end.
 
-  #[global] Instance showMetadata (md : metadata T) : Show (metadata T) :=
-    {| show := show_metadata |}.
+  #[global] Instance dshowMetadata (md : metadata T) : DShow (metadata T) :=
+    { dshow := dshow_metadata }.
 
   Definition show_unnamed_addr (u:unnamed_addr) : string :=
     match u with
@@ -731,7 +871,6 @@ tes on cstring on LLVMAst.v *)
 
   #[global] Instance showUnnamedAddr : Show unnamed_addr :=
     {| show := show_unnamed_addr |}.
-
 
   Definition show_tailcall (t:tailcall) : string :=
     match t with
@@ -744,10 +883,9 @@ tes on cstring on LLVMAst.v *)
     Instance showTailcall : Show tailcall :=
     {| show := show_tailcall |}.
 
-  Definition show_texp (x : texp T) : string :=
-    match x with
-    | (t, exp) => show t ++ " " ++ show_exp true exp
-      end.
+  Definition dshow_texp (x : texp T) : DString :=
+    let '(t, exp) := x in
+    dshow t @@ string_to_DString " " @@ dshow_exp true exp.
 
   Definition show_opt_space {A} (x:option A) : string :=
     match x with
@@ -761,16 +899,21 @@ tes on cstring on LLVMAst.v *)
     | _::_ => (concat c l) ++ " "
     end.
 
-  Definition show_call_arg '(te, atts) :=
-    let '(t, e) := (te:texp T) in
-    let attrs := concat_with_space " " (List.map show (atts:list param_attr)) in
-    (show (t:T)) ++ " " ++ attrs ++ (show_exp true (e:exp T)).
+  Definition show_call_arg (x : texp T * list param_attr) : DString :=
+    let '(te, atts) := x in
+    let '(t, e) := te in
+    let attrs := concat_DString (string_to_DString " ") (map dshow atts) @@ string_to_DString " " in
+    dshow t @@ string_to_DString  " " @@
+    attrs @@ dshow_exp true e.
 
-  Definition show_instr (i : instr T) : string
+  #[global] Instance dshowCallArg : DShow (texp T * list param_attr) :=
+    { dshow := show_call_arg }.
+
+  Definition dshow_instr (i : instr T) : DString
     := match i with
-       | INSTR_Comment s => "; " ++ s
+       | INSTR_Comment s => string_to_DString "; " @@  string_to_DString s
 
-       | INSTR_Op e => show e
+       | INSTR_Op e => dshow e
 
        | INSTR_Call fn args anns =>
            let tail := find_option ann_tail anns in
@@ -779,21 +922,21 @@ tes on cstring on LLVMAst.v *)
            let ret_attrs := filter_option ann_ret_attribute anns in
            let addrspace := find_option ann_addrspace anns in
            let fn_attrs := filter_option ann_fun_attribute anns in
-           (show_opt_prefix "" tail) ++ (show_opt_space tail)
-             ++
-             "call " ++
-             (concat_with_space " "
-                     ((map show_fast_math fast_math_flags)
-                        ++
-                        (show_opt_list cconv)
-                        ++
-                        (map show_param_attr ret_attrs)
-                        ++
-                        (show_opt_list addrspace)
-                     )
-             ) ++
-             show fn ++ "(" ++ (concat ", " (map show_call_arg args)) ++ ") " ++
-             (concat " " (map show_fn_attr fn_attrs))
+           string_to_DString (show_opt_prefix "" tail) @@ string_to_DString (show_opt_space tail)
+             @@ string_to_DString "call " @@
+             concat_DString (string_to_DString " ") (map (fun x => string_to_DString (show_fast_math x)) fast_math_flags)
+             @@
+             list_to_DString (show_opt_list cconv)
+             @@
+             DList_join (map show_param_attr ret_attrs)
+             @@
+             list_to_DString (show_opt_list addrspace) 
+
+             @@ string_to_DString " " @@
+             dshow fn @@ string_to_DString "(" @@
+             concat_DString (string_to_DString ", ") (map show_call_arg args) @@
+             string_to_DString ") " @@
+             concat_DString (string_to_DString " ") (map (fun x => string_to_DString (show_fn_attr x)) fn_attrs)
 
        | INSTR_Alloca t anns =>
            let inalloca := match find_option ann_inalloca anns with
@@ -803,7 +946,7 @@ tes on cstring on LLVMAst.v *)
            in
            let nb := find_option ann_num_elements anns in
            let align := find_option ann_align anns in
-           "alloca " ++ inalloca ++ show t ++ show_opt_prefix ", " nb ++ show_opt_prefix ", align " align
+           list_to_DString ["alloca " ; inalloca] @@ dshow t @@ dshow_opt_prefix (string_to_DString ", ") nb @@ string_to_DString (show_opt_prefix ", align " align)
 
        | INSTR_Load t ptr anns =>
            let volatile := match find_option ann_volatile anns with
@@ -813,12 +956,14 @@ tes on cstring on LLVMAst.v *)
            in
            let align := find_option ann_align anns in
            let meta := filter_option ann_metadata anns in
-           let meta_str := concatStr (List.map (fun '(m1, m2) =>
-                                                  ", "
-                                                    ++ (show_metadata (m1:metadata T)) ++ " " ++
-                                                    (show_metadata (m2:metadata T))) meta)
+           let meta_str := DList_join (map (fun '(m1, m2) =>
+                                                  string_to_DString ", "
+                                                    @@ dshow_metadata m1 @@ string_to_DString " " @@
+                                                    dshow_metadata m2)  meta)
            in
-           "load " ++ volatile ++ show t ++ ", " ++ show_texp ptr ++ (show_opt_prefix ", align " align) ++ meta_str
+           list_to_DString ["load "; volatile] @@ dshow t @@ string_to_DString ", " @@ dshow_texp ptr @@
+           string_to_DString (show_opt_prefix ", align " align) @@
+           meta_str
 
        | INSTR_Store tval ptr anns =>
            let volatile := match find_option ann_volatile anns with
@@ -828,51 +973,55 @@ tes on cstring on LLVMAst.v *)
            in
            let align := find_option ann_align anns in
            let meta := filter_option ann_metadata anns in
-           let meta_str := concatStr (List.map (fun '(m1, m2) =>
-                                                  ", "
-                                                    ++ (show_metadata (m1:metadata T)) ++ " " ++
-                                                    (show_metadata (m2:metadata T))) meta)
+           let meta_str := DList_join (map (fun '(m1, m2) =>
+                                                  string_to_DString ", "
+                                                    @@ dshow_metadata m1 @@ string_to_DString " " @@
+                                                    dshow_metadata m2) meta)
            in
-           "store " ++ volatile ++ show_texp tval ++ ", " ++ show_texp ptr ++ show_opt_prefix ", align " align ++ meta_str
+           string_to_DString "store " @@ string_to_DString volatile @@ dshow_texp tval @@
+           string_to_DString ", " @@ dshow_texp ptr @@ string_to_DString (show_opt_prefix ", align " align)
+                                                        @@ meta_str
 
        | INSTR_Fence syncscope ordering => let printable_sync := match syncscope with
                                                                  | None => ""
                                                                  | Some x => "[syncscope(""" ++ show x ++ """)]"
                                                                  end in
-                                           "fence " ++ printable_sync ++ show ordering  ++" ; yields void"
+                                          list_to_DString ["fence " ; printable_sync ] @@
+                                            dshow ordering @@
+                                            string_to_DString " ; yields void"
 
-       | INSTR_AtomicCmpXchg c => show_cmpxchg c
+       | INSTR_AtomicCmpXchg c => dshow c
 
        | INSTR_AtomicRMW a => show_atomic_rmw a
 
-       | INSTR_VAArg (va_list_and_arg_list) (t)  => "va_arg " ++ show va_list_and_arg_list ++ ", " ++ show t
+       | INSTR_VAArg va_list_and_arg_list t  =>
+           string_to_DString "va_arg " @@ dshow va_list_and_arg_list @@ string_to_DString ", " @@ dshow t
 
-       | INSTR_LandingPad => "skipping implementation at the moment"
+       | INSTR_LandingPad => string_to_DString "skipping implementation at the moment"
        end.
 
-  #[global] Instance showInstr : Show (instr T)
-    := {| show := show_instr |}.
+  #[global] Instance dshowInstr : DShow (instr T) := { dshow := dshow_instr }.
 
-  #[global] Instance showInstrId : Show instr_id
-    := {| show i :=
+  #[global] Instance dshowInstrId : DShow instr_id
+    := {| dshow i :=
          match i with
-         | IId raw => ("%" ++ show raw)%string
-         | IVoid n => ("void<" ++ show n ++ ">")%string
+         | IId raw => string_to_DString "%" @@ dshow raw
+         | IVoid n => string_to_DString "void<" @@ string_to_DString (show n) @@ string_to_DString ">"
          end
        |}.
 
-  Definition show_instr_id (inst : instr_id * instr T) : string
+  Definition dshow_instr_id (inst : instr_id * instr T) : DString
     :=
     let '(iid, i) := inst in
     match iid with
     | IId _ =>
-        (show iid ++ " = " ++ show i)%string
+        dshow iid @@ string_to_DString " = " @@ dshow i
     | IVoid n =>
-        show i
+        dshow i
     end.
 
-  #[global] Instance showInstrWithId : Show (instr_id * instr T)
-    := {| show := show_instr_id |}.
+  #[global] Instance dshowInstrWithId : DShow (instr_id * instr T)
+    := {| dshow := dshow_instr_id |}.
 
   Definition show_tint_literal (t : tint_literal) : string :=
     match t with
@@ -882,97 +1031,114 @@ tes on cstring on LLVMAst.v *)
   #[global] Instance showTintLiteral : Show tint_literal :=
     {| show := show_tint_literal |}.
 
-  Definition show_terminator (t : terminator T) : string
+  Definition dshow_terminator (t : terminator T) : DString
     := match t with
-       | TERM_Ret v => "ret " ++ show_texp v
-       | TERM_Ret_void => "ret void"
-       | TERM_Br te b1 b2 => "br " ++ show_texp te ++ ", label %" ++ show b1 ++ ", label %" ++ show b2
-       | TERM_Br_1 b => "br label %" ++ show b
-       | TERM_Switch v def_dest brs => concatStr["switch "; show_texp v; ", label %"; show def_dest;
-                                                 " ["; fold_left (fun str '(x, y) =>
-                                                                    str ++ show x ++ ", label %" ++ show y ++ " ") brs "";
-                                                 "]"]
+       | TERM_Ret v => string_to_DString "ret " @@ dshow_texp v
+       | TERM_Ret_void => string_to_DString "ret void"
+       | TERM_Br te b1 b2 =>
+           string_to_DString "br " @@ dshow_texp te @@
+           DList_join [string_to_DString ", label %" ; dshow b1 ; string_to_DString ", label %" ; dshow b2]
+       | TERM_Br_1 b => string_to_DString "br label %" @@ dshow b
 
-       | TERM_IndirectBr v brs => concatStr["indirectbr "; show_texp v; show brs]
-       | TERM_Resume v => "remove " ++ show_texp v
-       | TERM_Invoke fnptrval args to_label unwind_label => concatStr["invoke "; show fnptrval;
-                                                                      "( "; show args; "to label ";
-                                                                      show to_label; "unwind label ";
-                                                                      show unwind_label]
+       | TERM_Switch v def_dest brs => string_to_DString "switch " @@ dshow_texp v @@
+                                      string_to_DString ", label %" @@
+                                      dshow def_dest @@ string_to_DString " [" @@
+                                      fold_left (fun str '(x, y) => str @@ list_to_DString [show x; ", label %"] @@
+                                                                   dshow y @@ string_to_DString " ") brs DList_empty @@ string_to_DString "]"
 
-       | TERM_Unreachable => "unreachable"
+       | TERM_IndirectBr v brs => string_to_DString "indirectbr " @@ dshow_texp v @@
+                                   dshow brs
+
+       | TERM_Resume v => string_to_DString "remove " @@ dshow_texp v
+
+       | TERM_Invoke fnptrval args to_label unwind_label =>
+           string_to_DString "invoke " @@ dshow fnptrval @@
+             string_to_DString "( " @@ dshow args @@ string_to_DString "to label " @@
+             dshow to_label @@ string_to_DString "unwind label " @@ dshow unwind_label
+
+       | TERM_Unreachable => string_to_DString "unreachable"
        end.
 
-  #[global] Instance showTerminator : Show (terminator T)
-    := {| show := show_terminator |}.
+  #[global] Instance dshowTerminator : DShow (terminator T) := {dshow := dshow_terminator}.
 
-  Definition show_code (indent : string) (c : code T) : string
-    := concatStr (map (fun iid => indent ++ show_instr_id iid ++ newline) c).
+  Definition dshow_code (indent : string) (c : code T) : DString
+    := DList_join (map (fun iid => string_to_DString indent @@  dshow_instr_id iid @@ string_to_DString newline) c).
 
-  #[global] Instance showCode : Show (code T)
-    := {| show := show_code "    " |}.
+  #[global] Instance dshowCode : DShow (code T) := { dshow := dshow_code "    " }.
 
-  Definition show_block (indent : string) (b : block T) : string
+  Definition dnewline := string_to_DString newline.
+
+  Definition dshow_block (indent : string) (b : block T) : DString
     :=
-    let phis   := concatStr (map (fun '(l, p) => indent ++ "%" ++ show l ++ " = " ++ show p ++ newline) (blk_phis b)) in
-    let code   := show_code indent (blk_code b) in
-    let term   := indent ++ show (blk_term b) ++ newline in
-    show (blk_id b) ++ ":" ++ newline
-         ++ phis
-         ++ code
-         ++ term.
-  #[global] Instance showBlock: Show (block T) :=
-    {|
-      show := show_block "    "
-    |}.
+    let ind := string_to_DString indent in
+    let phis := DList_join (map (fun '(l, p) =>
+                                   ind @@
+                                     DList_join
+                                     [string_to_DString "%" ;
+                                      dshow l ;
+                                      string_to_DString " = " ;
+                                      dshow p ;
+                                      dnewline
+                              ])
+                              (blk_phis b)) in
+    let code   := dshow_code indent (blk_code b) in
+    let term   := DList_join [ind ; dshow (blk_term b) ; dnewline] in
+    DList_join [dshow (blk_id b); string_to_DString ":"; dnewline]
+         @@ phis
+         @@ code
+         @@ term.
 
-  Definition show_typ_instr (typ_instr: T * instr T) : string :=
+  #[global] Instance dshowBlock : DShow (block T) := { dshow := dshow_block  "    " }.
+
+  Definition dshow_typ_instr (typ_instr: T * instr T) : DString :=
     let (t, i) := typ_instr in
-    "(" ++ (show t) ++ ", " ++ (show i) ++ ")".
+    string_to_DString "(" @@ dshow t @@ string_to_DString ", " @@ dshow i @@ string_to_DString ")".
 
-  #[global] Instance showTypInstr: Show (T * instr T) :=
+  #[global] Instance dshowTypInstr: DShow (T * instr T) :=
     {|
-      show := show_typ_instr
+      dshow := dshow_typ_instr
     |}.
 
-  Definition show_arg (arg : local_id * T * list param_attr) : string
+  Definition dshow_arg (arg : local_id * T * list param_attr) : DString
     := let '(i, t, parameter_attributes) := arg in
-       show t ++ (match parameter_attributes with
-                  | [] => ""
-                  | _ => " " ++ concat " " (map (fun x => show x) (parameter_attributes))
-                  end) ++ " %" ++ show i.
+       dshow t @@
+         (match parameter_attributes with
+          | [] => string_to_DString ""
+          | _ => string_to_DString " " @@ concat_DString (string_to_DString " ") (map dshow (parameter_attributes))
+          end) @@ string_to_DString " %" @@ dshow i.
 
-  Definition show_arg_list (args : list (local_id * T * list param_attr)) (varargs:bool) : string
+  #[global] Instance dshowArg : DShow (local_id * T * list param_attr) :=
+    { dshow := dshow_arg }.
+
+  Definition dshow_arg_list (args : list (local_id * T * list param_attr)) (varargs:bool) : DString
     :=
     let vararg_str :=
       if Nat.eqb (List.length args) 0 then
-        (if varargs then "..." else "")
+        (if varargs then string_to_DString "..." else string_to_DString "")
       else
-        (if varargs then ", ..." else "")
+        (if varargs then string_to_DString ", ..." else string_to_DString "")
     in
-    let arg_str := concat ", " (map show_arg args)
+    let arg_str := concat_DString (string_to_DString ", ") (map dshow args)
     in
-      concatStr ["("; arg_str; vararg_str ; ")"].
-
-
-  (* TODO: REALLY?!? *)
-  Fixpoint zip {X Y} (xs : list X) (ys : list Y) : list (X * Y)
-    := match xs, ys with
-       | [], _ => []
-       | _, [] => []
-       | (x::xs), (y::ys) => (x, y) :: zip xs ys
-       end.
-
-  Fixpoint zip3 {X Y Z} (xs : list X) (ys : list Y) (zs : list Z) : list (X * Y *  Z)
-    := match xs, ys, zs with
-       | [], _, _ => []
-       | _, [], _ => []
-       | _, _, [] => []
-       | (x::xs), (y::ys), (z::zs) => (x, y, z) :: zip3 xs ys zs
-       end.
-
+    string_to_DString "(" @@ arg_str @@ vararg_str @@ string_to_DString ")".
 
 End ShowInstances.
+
+(* TODO: REALLY?!? *)
+Fixpoint zip {X Y} (xs : list X) (ys : list Y) : list (X * Y)
+  := match xs, ys with
+     | [], _ => []
+     | _, [] => []
+     | (x::xs), (y::ys) => (x, y) :: zip xs ys
+     end.
+
+Fixpoint zip3 {X Y Z} (xs : list X) (ys : list Y) (zs : list Z) : list (X * Y * Z)
+  := match xs, ys, zs with
+     | [], _, _ => []
+     | _, [], _ => []
+     | _, _, [] => []
+     | (x::xs), (y::ys), (z::zs) => (x, y, z) :: zip3 xs ys zs
+     end.
 
 (** Return empty string when None *)
 (** Adds a space -- is this the right place to do that? *)
@@ -982,15 +1148,25 @@ Definition maybe_to_string {X} (to_string : X -> string) (ox : option X) :=
   | Some x => ((to_string x) ++ " ")%string
   end.
 
-(** Return empty stringwhen None *)
+Definition maybe_to_dstring {X} (to_string : X -> DString) (ox : option X) :=
+  match ox with
+  | None => string_to_DString ""
+  | Some x => (to_string x) @@ string_to_DString " "
+  end.
+
+(** Return empty string when None *)
+
 Definition maybe_show {X} `{Show X} (ox : option X) : string :=
   maybe_to_string show ox.
 
-Definition show_definition (defn : definition typ (block typ * list (block typ))) : string
+Definition maybe_dshow {X} `{DShow X} (ox : option X) : DString :=
+  maybe_to_dstring dshow ox.
+
+Definition dshow_definition (defn : definition typ (block typ * list (block typ))) : DString
   :=
   let name  := defn.(df_prototype).(dc_name) in
   let ftype := defn.(df_prototype).(dc_type) in
-  let '(return_attributes, argument_attributes):= defn.(df_prototype).(dc_param_attrs) in
+  let '(return_attributes, argument_attributes) := defn.(df_prototype).(dc_param_attrs) in
 
   match ftype with
   | TYPE_Function ret_t args_t vararg =>
@@ -1001,17 +1177,18 @@ Definition show_definition (defn : definition typ (block typ * list (block typ))
          lead to tricky to catch problems otherwise.  *)
       let arg_length := List.length arg_names in
       if negb (Nat.eqb arg_length (List.length args_t) && (Nat.eqb arg_length (List.length argument_attributes)))
-      then "Function """ ++ show name ++ """ has mismatched arguments and argument attributes length"
+      then string_to_DString "Function """ @@ dshow name @@ string_to_DString """ has mismatched arguments and argument attributes length"
       else
         let args := zip3 arg_names args_t argument_attributes in
 
         let blocks :=
-          match df_instrs defn with
-          | (b, bs) => concat newline (map (show_block "    ") (b::bs))
-          end in
+          let '(b, bs) := df_instrs defn in
+          concat_DString dnewline (map dshow (b::bs))
+        in
 
-        let ret_attributes := concat " " (map (fun x => show x) (return_attributes)) in
-        let printable_ret_attrs := if ret_attributes then concatStr [" "; ret_attributes] else "" in
+        let ret_attributes := concat_DString (string_to_DString " ") (map (fun x => dshow x) (return_attributes)) @@
+        string_to_DString " " in
+        let printable_ret_attrs := ret_attributes in
 
         let linkage := maybe_show (dc_linkage defn.(df_prototype)) in
         let visibility := maybe_show (dc_visibility defn.(df_prototype)) in
@@ -1030,21 +1207,21 @@ Definition show_definition (defn : definition typ (block typ * list (block typ))
 
         let gc := maybe_show (dc_gc defn.(df_prototype)) in
 
-        concatStr ["define "; linkage; visibility ; dll_storage ;
-                   cconv ; printable_ret_attrs ; show ret_t; " @"; show name; show_arg_list args vararg;
-                   section ; align ; gc ; " {"; newline ;
-                   blocks;
-                   "}";
-                   newline]
+        DList_join [ list_to_DString ["define "; linkage; visibility; dll_storage ; cconv] @@
+                       printable_ret_attrs @@ dshow ret_t] @@ string_to_DString " @" @@ dshow name @@
+                     dshow_arg_list args vararg @@
+                     list_to_DString [section ; align ; gc ; " {"; newline] @@
+                     blocks @@
+                     list_to_DString ["}";  newline]
 
-  | _ => "Invalid type on function: " ++ show name
+  | _ => string_to_DString "Invalid type on function: " @@ dshow name
   end.
 
-Global Instance showDefinition: Show (definition typ (block typ * list (block typ))) :=
-  {| show := show_definition |}.
+#[global] Instance dshowDefinition: DShow (definition typ (block typ * list (block typ))) :=
+  {| dshow := dshow_definition |}.
 
 (* Why can I not make show functions implicit?  *)
-Definition show_declaration (decl: declaration typ) : string :=
+Definition dshow_declaration (decl: declaration typ) : DString :=
   let name := decl.(dc_name) in
   let (ret_attrs, args_attrs) := decl.(dc_param_attrs) in
   match decl.(dc_type) with
@@ -1072,33 +1249,35 @@ Definition show_declaration (decl: declaration typ) : string :=
         else
           (if vararg then ", ..." else "")
       in
-      concatStr ["declare "; link; vis; dll; cc;
-                 concatStr[intersperse " " (map show ret_attrs)]; " " ;
-
-                 show ret_t; " @"; show name;  "(";
-                 concat ", " (map (fun '(x, y) => concatStr[show x; " "; match y with
-                                                                      | [] => ""
-                                                                      | z :: tl => show z
-                                                                      end ])
-                                  (List.combine args_t args_attrs));
-                 vararg_str ;
-                 ")"; section; align; gc]
-  | _ => "Invalid type on function: " ++ show name
+      string_to_DString
+        (concatStr ["declare "; link; vis; dll; cc]) @@
+        DList_join [dintersperse (string_to_DString " ") (map dshow ret_attrs)] @@
+        string_to_DString " " @@
+        dshow ret_t @@ string_to_DString " @" @@ dshow name @@ string_to_DString "(" @@
+        dconcat (string_to_DString ", ") (map (fun '(x, y) =>
+                                                 DList_join
+                                                   [dshow x; string_to_DString " ";
+                                                    match y with
+                                                    | [] => string_to_DString ""
+                                                    | z :: tl => dshow z
+                                                    end ])
+                       (List.combine args_t args_attrs)) @@
+        string_to_DString vararg_str @@
+        string_to_DString ")" @@ string_to_DString section @@ string_to_DString align @@ string_to_DString gc
+  | _ => string_to_DString "Invalid type on function: " @@ dshow name
   end.
 
-Global Instance showDeclaration: Show (declaration typ) :=
-  {| show := show_declaration |}.
+#[global] Instance dshowDeclaration: DShow (declaration typ) :=
+  {| dshow := dshow_declaration |}.
 
-
-
-Definition show_global (g : global typ) : string :=
+Definition dshow_global (g : global typ) : DString :=
   let name  := g.(g_ident) in
   let gtype := g.(g_typ) in
   let linkage := maybe_show (g_linkage g) in
   let visibility := maybe_show (g_visibility g) in
   let dll_storage := maybe_show (g_dll_storage g) in
   let thread_local := maybe_show (g_thread_local_storage g) in
-  let g_exp := maybe_show g.(g_exp) in
+  let g_exp := maybe_dshow g.(g_exp) in
   let unnamed_addr := maybe_show (g_unnamed_addr g) in
   let addrspace := maybe_show (g_addrspace g) in
   let externally_initialized := if g.(g_externally_initialized) then "external " else "" in
@@ -1114,33 +1293,50 @@ Definition show_global (g : global typ) : string :=
       (fun a => concatStr ["align "; show a; " "])
       (g_align g) in
 
-  concatStr ["@"; show name ; " = " ; linkage ; visibility;
-             dll_storage ; thread_local;
-             unnamed_addr; addrspace;
-             externally_initialized; g_or_c;
-             show gtype; " "; g_exp;  section ; align].
+  DList_join
+    [string_to_DString "@"; dshow name; string_to_DString " = ";
+     string_to_DString linkage ; string_to_DString visibility;
+     string_to_DString dll_storage ; string_to_DString thread_local;
+     string_to_DString unnamed_addr; string_to_DString addrspace;
+     string_to_DString externally_initialized; string_to_DString g_or_c;
+     dshow gtype; string_to_DString " "; g_exp; string_to_DString section ; string_to_DString align
+    ].
 
-Global Instance showGlobal : Show (global typ) :=
-  {| show := show_global |}.
+#[global] Instance dshowGlobal : DShow (global typ) :=
+  {| dshow := dshow_global |}.
 
-Definition show_tle (tle : toplevel_entity typ (block typ * list (block typ))) : string
+Definition quoted_dstring (str : string) : DString
+  := string_to_DString (show str).
+
+Definition dshow_tle (tle : toplevel_entity typ (block typ * list (block typ))) : DString
   := match tle with
      (*Why is show_definition rather than show being used here*)
-     | TLE_Definition defn => show defn
-     | TLE_Comment msg => ";" ++ show msg (*What if the comment is multiple lines? *)
-     | TLE_Target tgt => "target triple = " ++  show tgt
-     | TLE_Datalayout layout => "target datalayout = " ++ show layout
-     | TLE_Source_filename s => "source_filename = " ++ show s
-     | TLE_Declaration decl => show decl
-     | TLE_Global g => show g
-     | TLE_Metadata id md => "!" ++ show id ++ " = " ++ show_metadata md (* Can't use implicit *)
-     | TLE_Type_decl id t => concatStr [show_ident id ;  " = type " ; show t ]
-     | TLE_Attribute_group i attrs => concatStr ["attributes #" ; show i ; " = { " ;
-                                                concat " " (map (fun x => show x) (attrs)) ; " }"  ]
+     | TLE_Definition defn => dshow defn
+     | TLE_Comment msg => string_to_DString ";" @@ quoted_dstring msg (*What if the comment is multiple lines? *)
+     | TLE_Target tgt => string_to_DString "target triple = " @@ quoted_dstring tgt
+     | TLE_Datalayout layout => string_to_DString "target datalayout = " @@ quoted_dstring layout
+     | TLE_Source_filename s => string_to_DString "source_filename = " @@ quoted_dstring s
+     | TLE_Declaration decl => dshow decl
+     | TLE_Global g => dshow g
+     | TLE_Metadata id md => string_to_DString "!" @@ dshow id @@ string_to_DString " = " @@ dshow_metadata md (* Can't use implicit *)
+     | TLE_Type_decl id t => DList_join [dshow_ident id ; string_to_DString " = type "; dshow t ]
+     | TLE_Attribute_group i attrs =>
+         DList_join
+           [string_to_DString "attributes #"; string_to_DString (show i); string_to_DString " = { " ;
+            dconcat (string_to_DString " ") (map (fun x => string_to_DString (show x)) (attrs)); string_to_DString " }"
+           ]
      end.
 
-Global Instance showTLE: Show (toplevel_entity typ (block typ  * list (block typ))) :=
-  {| show := show_tle |}.
+#[global] Instance dshowTLE: DShow (toplevel_entity typ (block typ  * list (block typ))) :=
+  {| dshow := dshow_tle |}.
 
-Global Instance showProg : Show (list (toplevel_entity typ (block typ * list (block typ)))) :=
-  {| show tles := concat (newline ++ newline) (map show_tle tles) |}.
+#[global] Instance dshowProg : DShow (list (toplevel_entity typ (block typ * list (block typ)))) :=
+  {| dshow tles := dconcat (dnewline @@ dnewline) (map dshow_tle tles) |}.
+
+Definition show_exp {T : Set} `{DShow T} (b: bool) (v : exp T) : string := show v.
+Definition showProg (p: list (toplevel_entity typ (block typ * list (block typ)))) : string := show p.
+Definition show_tle (tle : toplevel_entity typ (block typ * list (block typ))) : string := show tle.
+Definition show_typ (t : typ) : string := show t.
+
+#[global] Instance showTyp : Show typ :=
+  {| show := show_typ |}.
