src/coq/QC/QCShowTesting.v
@@ -1,0 +1,17 @@
+(** Testing show instances for Vellvm. Currently the show instances
+    seem to be causing stack overflows for larger programs. *)
+Require Import ExtrOcamlBasic.
+Require Import ExtrOcamlString.
+
+From QuickChick Require Import QuickChick.
+From Vellvm Require Import ShowAST ReprAST GenAST TopLevel LLVMAst DynamicValues QCVellvm.
+
+Extraction Blacklist String List Char Core Z Format.
+
+Extract Constant defNumTests    => "100".
+Extract Constant defSize    => "50".
+QCInclude "../../ml/*".
+QCInclude "../../ml/libvellvm/*".
+
+Extract Inlined Constant Error.failwith => "(fun _ -> raise)".
+QuickChick (forAll (run_GenLLVM gen_PROG) vellvm_agrees_with_clang).
